@prefix : <https://fast.ilabt.imec.be/ns/oslo-steps#> .
@prefix owl: <http://www.w3.org/2002/07/owl#> .
@prefix rdf: <http://www.w3.org/1999/02/22-rdf-syntax-ns#> .
@prefix xml: <http://www.w3.org/XML/1998/namespace> .
@prefix xsd: <http://www.w3.org/2001/XMLSchema#> .
@prefix rdfs: <http://www.w3.org/2000/01/rdf-schema#> .
@base <https://fast.ilabt.imec.be/ns/oslo-steps#> .

<https://fast.ilabt.imec.be/ns/oslo-steps#> rdf:type owl:Ontology ;
                                             owl:versionIRI <https://fast.ilabt.imec.be/ns/oslo-steps/0.2#> ;
                                             <http://purl.org/dc/terms/creator> <https://sven-lieber.org/profile#me> ;
                                             <http://purl.org/vocab/vann/preferredNamespacePrefix> "o-steps" ;
                                             <http://purl.org/vocab/vann/preferredNamespaceUri> "https://fast.ilabt.imec.be/ns/oslo-steps#" ;
                                             <http://purl.org/dc/terms/description> "This is the OSLO-STEPS vocabulary, aiming to describe steps of public services from a user perspective developed in the FAST project (http://www.project-fast.org)"@en ;
                                             rdfs:comment "Version 0.2: Added support for identifiable labels using skosXL. Version 0.1: an initial draft of the OSLO-STEPS vocabulary defined during the first year of the FAST project (http://www.project-fast.org)"@en ;
                                             owl:versionInfo "0.2"@en ;
                                             rdfs:label "OSLO-STEPS vocabulary"@en ;
                                             <http://purl.org/dc/terms/title> "OSLO-STEPS vocabulary"@en .

#################################################################
#    Annotation properties
#################################################################

###  http://www.w3.org/2004/02/skos/core#definition
<http://www.w3.org/2004/02/skos/core#definition> rdf:type owl:AnnotationProperty .


###  http://www.w3.org/ns/prov#definition
<http://www.w3.org/ns/prov#definition> rdf:type owl:AnnotationProperty .


#################################################################
#    Object Properties
#################################################################

###  http://purl.org/net/p-plan#correspondsToStep
<http://purl.org/net/p-plan#correspondsToStep> rdf:type owl:ObjectProperty ,
                                                        owl:FunctionalProperty ;
                                               rdfs:domain <http://purl.org/net/p-plan#Activity> ;
                                               rdfs:range <http://purl.org/net/p-plan#Step> ;
                                               rdfs:isDefinedBy <http://purl.org/net/p-plan#> ;
                                               rdfs:label "correspondsToStep"@en ;
                                               <http://www.w3.org/ns/prov#definition> "p-plan:correspondsToStep links a p-plan:Activity to its planned p-plan:Step"@en .


###  http://purl.org/net/p-plan#correspondsToVariable
<http://purl.org/net/p-plan#correspondsToVariable> rdf:type owl:ObjectProperty ,
                                                            owl:FunctionalProperty ;
                                                   rdfs:domain <http://purl.org/net/p-plan#Entity> ;
                                                   rdfs:range <http://purl.org/net/p-plan#Variable> ;
                                                   rdfs:isDefinedBy <http://purl.org/net/p-plan#> ;
                                                   rdfs:label "correspondsToVariable"@en ;
                                                   <http://www.w3.org/ns/prov#definition> "p-plan:correspondsToVariable binds a p-plan:Entity (used by a p-plan:Activity in the execution of a plan) to the p-plan:Variable it represented it in the p-plan:Plan."@en .


###  http://purl.org/net/p-plan#isDecomposedAsPlan
<http://purl.org/net/p-plan#isDecomposedAsPlan> rdf:type owl:ObjectProperty ;
                                                rdfs:domain <http://purl.org/net/p-plan#MultiStep> ;
                                                rdfs:range <http://purl.org/net/p-plan#Plan> ;
                                                rdfs:isDefinedBy <http://purl.org/net/p-plan#> ;
                                                rdfs:label "isDecomposedAsPlan"@en ;
                                                <http://www.w3.org/ns/prov#definition> "The p-plan:isDecomposedAsPlan relationship binds a p-plan:MultiStep to the p-plan:Plan holding the definition of that step. That is, p-plan:isDecomposedAsPlan links the MultiStep to the Plan sptecification where it is decomposed."@en .


###  http://purl.org/net/p-plan#isStepOfPlan
<http://purl.org/net/p-plan#isStepOfPlan> rdf:type owl:ObjectProperty ;
                                          rdfs:domain <http://purl.org/net/p-plan#Step> ;
                                          rdfs:range <http://purl.org/net/p-plan#Plan> ;
                                          rdfs:isDefinedBy <http://purl.org/net/p-plan#> ;
                                          rdfs:label "isStepOfPlan"@en ;
                                          <http://www.w3.org/ns/prov#definition> "p-plan:isStepOfPlan links a p-plan:Step to the p-plan:Plan which it corresponds to."@en .


###  http://purl.org/net/p-plan#isSubPlanOfPlan
<http://purl.org/net/p-plan#isSubPlanOfPlan> rdf:type owl:ObjectProperty ;
                                             rdfs:subPropertyOf owl:topObjectProperty ;
                                             rdfs:domain <http://purl.org/net/p-plan#Plan> ;
                                             rdfs:range <http://purl.org/net/p-plan#Plan> ;
                                             rdfs:isDefinedBy <http://purl.org/net/p-plan#> ;
                                             rdfs:label "isSubPlanOfPlan"@en ;
                                             <http://www.w3.org/ns/prov#definition> "A p-plan:Plan may be a subplan of another bigger p-plan:Plan. p-plan:isSubPlanOfPlan is used to state the link among the two different plans. Note that if p1 is a p-plan:subPlan of p2, p1will not necessarily be a step of p2. A multistep will represent p1 in p2, and link to p1 with the p-plan.hasStepDecomposition relationship."@en .


###  http://www.w3.org/2008/05/skos-xl#altLabel
<http://www.w3.org/2008/05/skos-xl#altLabel> rdf:type owl:ObjectProperty ;
                                             rdfs:range <http://www.w3.org/2008/05/skos-xl#Label> ;
                                             rdfs:comment "If C skosxl:altLabel L and L skosxl:literalForm V, then X skos:altLabel V."@en ;
                                             rdfs:isDefinedBy <http://www.w3.org/2008/05/skos-xl> ;
                                             rdfs:label "alternative label"@en ;
                                             rdfs:seeAlso <http://www.w3.org/2004/02/skos/core#altLabel> ;
                                             <http://www.w3.org/2004/02/skos/core#definition> "The property skosxl:altLabel is used to associate an skosxl:Label with a skos:Concept. The property is analogous to skos:altLabel."@en .


###  http://www.w3.org/2008/05/skos-xl#prefLabel
<http://www.w3.org/2008/05/skos-xl#prefLabel> rdf:type owl:ObjectProperty ;
                                              rdfs:range <http://www.w3.org/2008/05/skos-xl#Label> ;
                                              rdfs:comment "If C skosxl:prefLabel L and L skosxl:literalForm V, then X skos:prefLabel V."@en ;
                                              rdfs:isDefinedBy <http://www.w3.org/2008/05/skos-xl> ;
                                              rdfs:label "preferred label"@en ;
                                              rdfs:seeAlso <http://www.w3.org/2004/02/skos/core#prefLabel> ;
                                              <http://www.w3.org/2004/02/skos/core#definition> "The property skosxl:prefLabel is used to associate an skosxl:Label with a skos:Concept. The property is analogous to skos:prefLabel."@en .


###  https://fast.ilabt.imec.be/ns/oslo-steps#hasDescription
:hasDescription rdf:type owl:ObjectProperty ;
                rdfs:domain <http://purl.org/net/p-plan#Step> ;
                rdfs:range <http://www.w3.org/2008/05/skos-xl#Label> .


###  https://fast.ilabt.imec.be/ns/oslo-steps#hasStateShape
:hasStateShape rdf:type owl:ObjectProperty ;
               rdfs:domain :State ;
               rdfs:range :StateShape ;
               rdfs:comment "Links a o-steps:State to a description of the state as o-steps:StateShape."@en ;
               rdfs:isDefinedBy <https://fast.ilabt.imec.be/ns/oslo-steps#> ;
               rdfs:label "hasStateShape"@en .


###  https://fast.ilabt.imec.be/ns/oslo-steps#producesState
:producesState rdf:type owl:ObjectProperty ;
               rdfs:domain :Step ;
               rdfs:range :State ;
               rdfs:comment "o-steps:producesState binds a o-steps:Step to the o-steps:State the step produces."@en ;
               rdfs:isDefinedBy <https://fast.ilabt.imec.be/ns/oslo-steps#> ;
               rdfs:label "producesState"@en .


###  https://fast.ilabt.imec.be/ns/oslo-steps#requiresState
:requiresState rdf:type owl:ObjectProperty ;
               rdfs:domain :Step ;
               rdfs:range :State ;
               rdfs:comment "o-steps:requiresState binds a o-steps:Step to the o-steps:State the step requires to produce the state bound via o-steps:producesState."@en ;
               rdfs:isDefinedBy <https://fast.ilabt.imec.be/ns/oslo-steps#> ;
               rdfs:label "requiresState"@en .


#################################################################
#    Data properties
#################################################################

###  http://www.w3.org/2008/05/skos-xl#literalForm
<http://www.w3.org/2008/05/skos-xl#literalForm> rdf:type owl:DatatypeProperty ;
                                                rdfs:domain <http://www.w3.org/2008/05/skos-xl#Label> ;
                                                rdfs:comment "If two instances of the class skosxl:Label have the same literal form, they are not necessarily the same resource."@en ,
                                                             "The range of skosxl:literalForm is the class of RDF plain literals."@en ;
                                                rdfs:isDefinedBy <http://www.w3.org/2008/05/skos-xl> ;
                                                rdfs:label "literal form"@en ;
                                                <http://www.w3.org/2004/02/skos/core#definition> "The property skosxl:literalForm is used to give the literal form of an skosxl:Label."@en .


#################################################################
#    Classes
#################################################################

###  http://purl.org/net/p-plan#Activity
<http://purl.org/net/p-plan#Activity> rdf:type owl:Class .


###  http://purl.org/net/p-plan#Bundle
<http://purl.org/net/p-plan#Bundle> rdf:type owl:Class ;
                                    rdfs:subClassOf <http://purl.org/net/p-plan#Entity> ,
                                                    <http://www.w3.org/ns/prov#Bundle> ;
                                    rdfs:comment "A p-plan:Bundle is a specific type of prov:Bundle that contains the provenance assertions of the execution of a p-plan:Plan"@en ;
                                    rdfs:isDefinedBy <http://purl.org/net/p-plan#> ;
                                    rdfs:label "Bundle"@en .


###  http://purl.org/net/p-plan#Entity
<http://purl.org/net/p-plan#Entity> rdf:type owl:Class .


###  http://purl.org/net/p-plan#MultiStep
<http://purl.org/net/p-plan#MultiStep> rdf:type owl:Class .


###  http://purl.org/net/p-plan#Plan
<http://purl.org/net/p-plan#Plan> rdf:type owl:Class ;
                                  rdfs:subClassOf <http://purl.org/net/p-plan#Entity> ,
                                                  <http://www.w3.org/ns/prov#Plan> ;
                                  rdfs:isDefinedBy <http://purl.org/net/p-plan#> ;
                                  rdfs:label "Plan"@en ;
                                  <http://www.w3.org/ns/prov#definition> "A p-plan:Plan is a specific type of prov:Plan. It is composed of smaller steps that use and produce Variables."@en .


###  http://purl.org/net/p-plan#Step
<http://purl.org/net/p-plan#Step> rdf:type owl:Class ;
                                  rdfs:isDefinedBy <http://purl.org/net/p-plan#> ;
                                  rdfs:label "Step"@en ;
                                  <http://www.w3.org/ns/prov#definition> "A p-plan:Step represents the planned execution activity"@en .


###  http://purl.org/net/p-plan#Variable
<http://purl.org/net/p-plan#Variable> rdf:type owl:Class ;
                                      rdfs:isDefinedBy <http://purl.org/net/p-plan#> ;
                                      rdfs:label "Variable"@en ;
                                      <http://www.w3.org/ns/prov#definition> "A p-plan:Variable represents a description of the input of the planned Activity (p-plan:Step)"@en .


###  http://www.w3.org/2004/02/skos/core#Collection
<http://www.w3.org/2004/02/skos/core#Collection> rdf:type owl:Class ;
                                                 owl:disjointWith <http://www.w3.org/2008/05/skos-xl#Label> .


###  http://www.w3.org/2004/02/skos/core#Concept
<http://www.w3.org/2004/02/skos/core#Concept> rdf:type owl:Class ;
                                              owl:disjointWith <http://www.w3.org/2008/05/skos-xl#Label> .


###  http://www.w3.org/2004/02/skos/core#ConceptScheme
<http://www.w3.org/2004/02/skos/core#ConceptScheme> rdf:type owl:Class ;
                                                    owl:disjointWith <http://www.w3.org/2008/05/skos-xl#Label> .


###  http://www.w3.org/2008/05/skos-xl#Label
<http://www.w3.org/2008/05/skos-xl#Label> rdf:type owl:Class ;
                                          rdfs:subClassOf [ rdf:type owl:Restriction ;
                                                            owl:onProperty <http://www.w3.org/2008/05/skos-xl#literalForm> ;
                                                            owl:cardinality "1"^^xsd:nonNegativeInteger
                                                          ] ;
                                          rdfs:isDefinedBy <http://www.w3.org/2008/05/skos-xl> ;
                                          rdfs:label "Label"@en ;
                                          <http://www.w3.org/2004/02/skos/core#definition> "A special class of lexical entities."@en .


###  http://www.w3.org/ns/prov#Bundle
<http://www.w3.org/ns/prov#Bundle> rdf:type owl:Class .


###  http://www.w3.org/ns/prov#Plan
<http://www.w3.org/ns/prov#Plan> rdf:type owl:Class .


###  http://www.w3.org/ns/shacl#NodeShape
<http://www.w3.org/ns/shacl#NodeShape> rdf:type owl:Class ;
                                       rdfs:comment "A node shape is a shape that specifies constraint that need to be met with respect to focus nodes."@en ;
                                       rdfs:isDefinedBy <http://www.w3.org/ns/shacl#> ;
                                       rdfs:label "Node shape"@en .


###  http://www.w3.org/ns/shacl#PropertyShape
<http://www.w3.org/ns/shacl#PropertyShape> rdf:type owl:Class ;
                                           rdfs:comment "A property shape is a shape that specifies constraints on the values of a focus node for a given property or path."@en ;
                                           rdfs:isDefinedBy <http://www.w3.org/ns/shacl#> ;
                                           rdfs:label "Property shape"@en .


###  https://fast.ilabt.imec.be/ns/oslo-steps#Bundle
:Bundle rdf:type owl:Class ;
        rdfs:subClassOf <http://purl.org/net/p-plan#Bundle> ;
        rdfs:comment "A o-steps:Bundle is a specific type of p-plan:Bundle that contains the provenance assertions of the execution of a o-steps:Plan"@en ;
        rdfs:isDefinedBy <https://fast.ilabt.imec.be/ns/oslo-steps#> ;
        rdfs:label "Bundle"@en .


###  https://fast.ilabt.imec.be/ns/oslo-steps#Plan
:Plan rdf:type owl:Class ;
      rdfs:subClassOf <http://purl.org/net/p-plan#Plan> ;
      rdfs:comment "A o-steps:Plan is a specific type of p-plan:Plan. It is composed of smaller steps that require and produce states."@en ;
      rdfs:isDefinedBy <https://fast.ilabt.imec.be/ns/oslo-steps#> ;
      rdfs:label "Plan"@en .


###  https://fast.ilabt.imec.be/ns/oslo-steps#State
:State rdf:type owl:Class ;
       rdfs:subClassOf <http://purl.org/net/p-plan#Variable> ;
       rdfs:comment "A state in the sense of a particular condition something is in. In our case a state could be represented as a set of RDF statements."@en ;
       rdfs:isDefinedBy <https://fast.ilabt.imec.be/ns/oslo-steps#> ;
       rdfs:label "State"@en .


###  https://fast.ilabt.imec.be/ns/oslo-steps#StateShape
:StateShape rdf:type owl:Class ;
            rdfs:subClassOf <http://www.w3.org/ns/shacl#NodeShape> ;
            rdfs:comment "A state shape is a shape that specifies a set of triples representing a state, and is described as constraints."@en ;
            rdfs:isDefinedBy <https://fast.ilabt.imec.be/ns/oslo-steps#> ;
            rdfs:label "State shape"@en .


###  https://fast.ilabt.imec.be/ns/oslo-steps#Step
:Step rdf:type owl:Class ;
      rdfs:subClassOf <http://purl.org/net/p-plan#Step> ;
      rdfs:comment "The Workflow Coalition defines a step as: 'A description of a piece of work that forms one logical step within a process'. Furthermore, such a step may be either a workflow, or the smallest unit of work which is scheduled based on pre/post-conditions (states)."@en ;
      rdfs:isDefinedBy <https://fast.ilabt.imec.be/ns/oslo-steps#> ;
      rdfs:label "Step"@en .


###  Generated by the OWL API (version 4.2.8.20170104-2310) https://github.com/owlcs/owlapi
